SP1Chips/BitwiseChip.lean
@@ -5,58 +5,169 @@ open LeanRV32D.Functions Sail
 
 namespace BitwiseChip
 
-
-def constraints
-  (Main : Vector BabyBear 23)
-  : SP1ConstraintList :=
-  let E0 : BabyBear := Main[22] - 1
-  let E2 : BabyBear := Main[22] * E0
-  let E4 : BabyBear := Main[3] + 4
-  let E6 : BabyBear := 16384 * Main[1]
-  let E8 : BabyBear := E6 + Main[2]
-  [ .assertZero E2
-  ]
-  ++ (AddOperation.constraints #v[Main[11], Main[12], Main[16], Main[17], Main[20], Main[21], Main[22]])
-  ++ (CPUState.constraints
-      { shard := Main[0]
-      , clk_high_limb := Main[1]
-      , clk_low_limb := Main[2]
-      , pc := Main[3] }
-      E4
-      4
-      Main[22])
-  ++ (RTypeReader.constraints
+def constraints (Main : Vector BabyBear 33) : SP1ConstraintList :=
+  let E0 : BabyBear := Main[30] + Main[31]
+  let E1 : BabyBear := E0 + Main[32]
+  let E2 : BabyBear := Main[30] - 1
+  let E3 : BabyBear := Main[30] * E2
+  let E4 : BabyBear := Main[31] - 1
+  let E5 : BabyBear := Main[31] * E4
+  let E6 : BabyBear := Main[32] - 1
+  let E7 : BabyBear := Main[32] * E6
+  let E8 : BabyBear := E1 - 1
+  let E9 : BabyBear := E1 * E8
+  let E10 : BabyBear := Main[30] * 2
+  let E11 : BabyBear := Main[31] * 1
+  let E12 : BabyBear := E10 + E11
+  let E13 : BabyBear := Main[32] * 0
+  let E14 : BabyBear := E12 + E13
+  let E15 : BabyBear := Main[30] * 3
+  let E16 : BabyBear := Main[31] * 4
+  let E17 : BabyBear := E15 + E16
+  let E18 : BabyBear := Main[32] * 5
+  let E19 : BabyBear := E17 + E18
+  let ⟨⟨⟨[E20, E21]⟩, _⟩, CS0⟩ := BitwiseU16Operation.constraints
+    #v[Main[11], Main[12]] #v[Main[17], Main[18]]
+    { a_low_bytes := { low_bytes := #v[Main[22], Main[23]] },
+      bitwise_operation := { result := #v[Main[26], Main[27], Main[28], Main[29]] },
+      b_low_bytes := { low_bytes := #v[Main[24], Main[25]] } }
+      E14
+      E1
+  let E22 : BabyBear := Main[3] + 4
+  let CS1 : List SP1Constraint := CPUState.constraints
+    { clk_0_16 := Main[2],
+      clk_16_24 := Main[1],
+      clk_high := Main[0], pc := Main[3] } E22 8 E1
+  let E23 : BabyBear := Main[1] * 65536
+  let E24 : BabyBear := Main[2] + E23
+  let CS2 : List SP1Constraint := ALUTypeReader.constraints
     Main[0]
-    E8
-    -- Main[3]
-    -- 0
-    #v[Main[20], Main[21]]
-    { op_a := Main[4]
-    , op_a_memory :=
-        { prev_value := #v[Main[5], Main[6]]
-        , access_timestamp :=
-            { prev_clk := Main[7]
-            , diff_low_limb := Main[8]
-            }
-        }
-    , op_a_0 := Main[9]
-    , op_b := Main[10]
-    , op_b_memory :=
-        { prev_value := #v[Main[11], Main[12]]
-        , access_timestamp :=
-            { prev_clk := Main[13]
-            , diff_low_limb := Main[14]
-            }
-        }
-    , op_c := Main[15]
-    , op_c_memory :=
-        { prev_value := #v[Main[16], Main[17]]
-        , access_timestamp :=
-            { prev_clk := Main[18]
-            , diff_low_limb := Main[19]
-            }
-        }
-    }
-    Main[22])
+    E24
+    Main[3]
+    E19
+    #v[E20, E21]
+    { imm_c := Main[21],
+      op_a := Main[4],
+      op_a_0 := Main[9],
+      op_a_memory :=
+        { access_timestamp := { diff_low_limb := Main[8], prev_low := Main[7] },
+          prev_value := #v[Main[5], Main[6]] },
+      op_b := Main[10],
+      op_b_memory :=
+        { access_timestamp := { diff_low_limb := Main[14], prev_low := Main[13] },
+          prev_value := #v[Main[11], Main[12]] },
+      op_c := #v[Main[15], Main[16]],
+      op_c_memory :=
+        { access_timestamp := { diff_low_limb := Main[20], prev_low := Main[19] },
+          prev_value := #v[Main[17], Main[18]] } } E1
+  [
+    .assertZero E3,
+    .assertZero E5,
+    .assertZero E7,
+    .assertZero E9
+  ] ++ CS0 ++ CS1 ++ CS2
+
+/-- `is_real` for the op is the sum of the individual opcodes. -/
+def is_real (Main : Vector BabyBear 33) : BabyBear :=
+  Main[30] + Main[31] + Main[32]
+
+section and
+
+def Word.bitvec_of_babybear (w : Word BabyBear) : BitVec 32 :=
+  BitVec.ofNatLT ((w[0] + w[1] * 65536) % 2^32) (by omega)
+
+def main_output (Main : Vector BabyBear 33) : BitVec 32 :=
+  let E0 : BabyBear := Main[30] + Main[31]
+  let E1 : BabyBear := E0 + Main[32]
+  let E2 : BabyBear := Main[30] - 1
+  let E3 : BabyBear := Main[30] * E2
+  let E4 : BabyBear := Main[31] - 1
+  let E5 : BabyBear := Main[31] * E4
+  let E6 : BabyBear := Main[32] - 1
+  let E7 : BabyBear := Main[32] * E6
+  let E8 : BabyBear := E1 - 1
+  let E9 : BabyBear := E1 * E8
+  let E10 : BabyBear := Main[30] * 2
+  let E11 : BabyBear := Main[31] * 1
+  let E12 : BabyBear := E10 + E11
+  let E13 : BabyBear := Main[32] * 0
+  let E14 : BabyBear := E12 + E13
+  let E15 : BabyBear := Main[30] * 3
+  let E16 : BabyBear := Main[31] * 4
+  let E17 : BabyBear := E15 + E16
+  let E18 : BabyBear := Main[32] * 5
+  let E19 : BabyBear := E17 + E18
+  let ⟨⟨⟨[E20, E21]⟩, _⟩, CS0⟩ := BitwiseU16Operation.constraints
+    #v[Main[11], Main[12]] #v[Main[17], Main[18]]
+    { a_low_bytes := { low_bytes := #v[Main[22], Main[23]] },
+      bitwise_operation := { result := #v[Main[26], Main[27], Main[28], Main[29]] },
+      b_low_bytes := { low_bytes := #v[Main[24], Main[25]] } }
+      E14
+      E1
+  BitVec.ofNat 32 (E20 + E21 * 65536)
+
+def sp1_bitwise
+    (Main : Vector BabyBear 33)
+    (rd rs1 rs2 : regidx) :
+    SailM Unit := do
+  writeReg Register.nextPC (BitVec.addInt (← readReg Register.PC) 4)
+  let _rs1_value ← rX_bits rs1
+  let _rs2_value ← rX_bits rs2
+  wX_bits rd (main_output Main)
+
+def spec_and (rd rs1 rs2 : regidx) : SailM Unit := do
+  writeReg Register.nextPC (BitVec.addInt (← readReg Register.PC) 4)
+  let _ ← execute_RTYPE rs2 rs1 rd rop.AND
+  pure ()
+
+def spec_or (rd rs1 rs2 : regidx) : SailM Unit := do
+  writeReg Register.nextPC (BitVec.addInt (← readReg Register.PC) 4)
+  let _ ← execute_RTYPE rs2 rs1 rd rop.OR
+  pure ()
+
+def spec_xor (rd rs1 rs2 : regidx) : SailM Unit := do
+  writeReg Register.nextPC (BitVec.addInt (← readReg Register.PC) 4)
+  let _ ← execute_RTYPE rs2 rs1 rd rop.XOR
+  pure ()
+
+theorem sp1_bitwise_eq_spec_xor
+    (Main : Vector BabyBear 33)
+    (cstrs : (constraints Main).allHold)
+    (rd rs1 rs2 : regidx)
+    (h_is_and : Main[30] = 1) :
+    sp1_bitwise Main rd rs1 rs2 = spec_xor rd rs1 rs2 := by
+  unfold sp1_bitwise spec_xor
+
+  have spare_cstrs : (constraints Main).allHold := cstrs
+
+  have h30_0 : Main[30] = 1 := sorry
+  have h31_0 : Main[31] = 0 := sorry
+  have h32_0 : Main[32] = 0 := sorry
+
+  simp only [SP1ConstraintList.allHold, constraints, BabyBearPrime, Fin.isValue, mul_one, mul_zero,
+    add_zero, WORD_SIZE, List.cons_append, List.nil_append, List.append_assoc] at cstrs
+  obtain ⟨h31, h31, h32, h_add_3, hop, hreg⟩ := cstrs
+  simp [- SP1Constraint.toProp_send_byte] at hreg
+
+  simp [h30_0, h31_0, h32_0, sub_eq_zero] at *
+  obtain ⟨⟨hbd0, h_xor0⟩, ⟨hbd1, h_xor1⟩, ⟨hbd2, h_xor2⟩, ⟨hbd3, h_xor3⟩, h_cpu, h_alu⟩ := hreg
+
+  simp [main_output, BitwiseU16Operation.constraints, execute_RTYPE]
+
+  have read_b := ALUTypeReader.read_b_fun _ rs1 h_alu
+  have read_c := ALUTypeReader.read_c_fun _ rs2 h_alu
+  rw [read_b, read_c]
+
+  refine bind_congr fun _ => ?_
+  refine bind_congr fun _ => ?_
+  refine congr_arg (wX_bits rd) ?_
+
+  simp
+  -- simp
+  clear read_b read_c h_alu h_cpu
+
+  sorry
+
+end and
 
 end BitwiseChip
