SP1Operations/BitwiseOperation.lean
@@ -22,8 +22,8 @@ namespace BitwiseOperation
 open ByteOpcode
 
 def constraints
-  (a : Vector BabyBear WORD_BYTE_SIZE)
-  (b : Vector BabyBear WORD_BYTE_SIZE)
+  (a : ByteWord BabyBear)
+  (b : ByteWord BabyBear)
   (cols : BitwiseOperation)
   (opcode : BabyBear)
   (is_real : BabyBear)
@@ -35,26 +35,26 @@ def constraints
     .send (.byte (ByteOpcode.ofNat opcode) cols.result[3] a[3] b[3]) is_real
   ]
 
-def spec (a b : Vector BabyBear WORD_BYTE_SIZE)
+def spec (a b : ByteWord BabyBear)
     (cols : BitwiseOperation) (opcode : BabyBear) : Prop :=
   if ByteOpcode.ofNat opcode = .AND then (
-    ((cols.result[0] < 256 ∧ a[0] < 256 ∧ b[0] < 256) → cols.result[0] = a[0] &&& b[0]) ∧
-    ((cols.result[1] < 256 ∧ a[1] < 256 ∧ b[1] < 256) → cols.result[1] = a[1] &&& b[1]) ∧
-    ((cols.result[2] < 256 ∧ a[2] < 256 ∧ b[2] < 256) → cols.result[2] = a[2] &&& b[2]) ∧
-    ((cols.result[3] < 256 ∧ a[3] < 256 ∧ b[3] < 256) → cols.result[3] = a[3] &&& b[3])
+    ((cols.result[0] < 256 ∧ a[0] < 256 ∧ b[0] < 256) ∧ cols.result[0] = a[0] &&& b[0]) ∧
+    ((cols.result[1] < 256 ∧ a[1] < 256 ∧ b[1] < 256) ∧ cols.result[1] = a[1] &&& b[1]) ∧
+    ((cols.result[2] < 256 ∧ a[2] < 256 ∧ b[2] < 256) ∧ cols.result[2] = a[2] &&& b[2]) ∧
+    ((cols.result[3] < 256 ∧ a[3] < 256 ∧ b[3] < 256) ∧ cols.result[3] = a[3] &&& b[3])
   ) else if ByteOpcode.ofNat opcode = .OR then (
-    ((cols.result[0] < 256 ∧ a[0] < 256 ∧ b[0] < 256) → cols.result[0] = a[0] ||| b[0]) ∧
-    ((cols.result[1] < 256 ∧ a[1] < 256 ∧ b[1] < 256) → cols.result[1] = a[1] ||| b[1]) ∧
-    ((cols.result[2] < 256 ∧ a[2] < 256 ∧ b[2] < 256) → cols.result[2] = a[2] ||| b[2]) ∧
-    ((cols.result[3] < 256 ∧ a[3] < 256 ∧ b[3] < 256) → cols.result[3] = a[3] ||| b[3])
+    ((cols.result[0] < 256 ∧ a[0] < 256 ∧ b[0] < 256) ∧ cols.result[0] = a[0] ||| b[0]) ∧
+    ((cols.result[1] < 256 ∧ a[1] < 256 ∧ b[1] < 256) ∧ cols.result[1] = a[1] ||| b[1]) ∧
+    ((cols.result[2] < 256 ∧ a[2] < 256 ∧ b[2] < 256) ∧ cols.result[2] = a[2] ||| b[2]) ∧
+    ((cols.result[3] < 256 ∧ a[3] < 256 ∧ b[3] < 256) ∧ cols.result[3] = a[3] ||| b[3])
   ) else if ByteOpcode.ofNat opcode = .XOR then (
-    ((cols.result[0] < 256 ∧ a[0] < 256 ∧ b[0] < 256) → cols.result[0] = a[0] ^^^ b[0]) ∧
-    ((cols.result[1] < 256 ∧ a[1] < 256 ∧ b[1] < 256) → cols.result[1] = a[1] ^^^ b[1]) ∧
-    ((cols.result[2] < 256 ∧ a[2] < 256 ∧ b[2] < 256) → cols.result[2] = a[2] ^^^ b[2]) ∧
-    ((cols.result[3] < 256 ∧ a[3] < 256 ∧ b[3] < 256) → cols.result[3] = a[3] ^^^ b[3])
+    ((cols.result[0] < 256 ∧ a[0] < 256 ∧ b[0] < 256) ∧ cols.result[0] = a[0] ^^^ b[0]) ∧
+    ((cols.result[1] < 256 ∧ a[1] < 256 ∧ b[1] < 256) ∧ cols.result[1] = a[1] ^^^ b[1]) ∧
+    ((cols.result[2] < 256 ∧ a[2] < 256 ∧ b[2] < 256) ∧ cols.result[2] = a[2] ^^^ b[2]) ∧
+    ((cols.result[3] < 256 ∧ a[3] < 256 ∧ b[3] < 256) ∧ cols.result[3] = a[3] ^^^ b[3])
   ) else True
 
-lemma constraints_imp_spec (a b : Vector BabyBear WORD_BYTE_SIZE)
+lemma constraints_imp_spec (a b : ByteWord BabyBear)
     (cols : BitwiseOperation) (opcode is_real : BabyBear)
     (h0 : is_real ≠ 0)
     (h : (cols.constraints a b opcode is_real).allHold) :
@@ -68,52 +68,38 @@ lemma constraints_imp_spec (a b : Vector BabyBear WORD_BYTE_SIZE)
   · simpa [h0, h3] using h
   simp [h1, h2, h3]
 
-lemma eq_and_of_constraints (a b : Vector BabyBear WORD_BYTE_SIZE) (cols : BitwiseOperation)
-    (i : Fin WORD_BYTE_SIZE) (ha : a[i] < 256) (hb : b[i] < 256) (hc : cols.result[i] < 256)
-    (h : (cols.constraints a b 0 1).allHold) :
+lemma eq_and_of_constraints (a b : ByteWord BabyBear) (cols : BitwiseOperation)
+    (i : Fin WORD_BYTE_SIZE) (h : (cols.constraints a b 0 1).allHold) :
     cols.result[i] = a[i] &&& b[i] := by
   have := constraints_imp_spec a b cols _ _ one_ne_zero h
   simp [spec] at this
-  exact match i with
-  | 0 => this.1 hc ha hb
-  | 1 => this.2.1 hc ha hb
-  | 2 => this.2.2.1 hc ha hb
-  | 3 => this.2.2.2 hc ha hb
+  match i with | 0 => aesop | 1 => aesop | 2 => aesop | 3 => aesop
 
-lemma eq_or_of_constraints (a b : Vector BabyBear WORD_BYTE_SIZE) (cols : BitwiseOperation)
-    (i : Fin WORD_BYTE_SIZE) (ha : a[i] < 256) (hb : b[i] < 256) (hc : cols.result[i] < 256)
-    (h : (cols.constraints a b 1 1).allHold) :
+lemma eq_or_of_constraints (a b : ByteWord BabyBear) (cols : BitwiseOperation)
+    (i : Fin WORD_BYTE_SIZE) (h : (cols.constraints a b 1 1).allHold) :
     cols.result[i] = a[i] ||| b[i] := by
   have := constraints_imp_spec a b cols _ _ one_ne_zero h
   simp [spec] at this
-  exact match i with
-  | 0 => this.1 hc ha hb
-  | 1 => this.2.1 hc ha hb
-  | 2 => this.2.2.1 hc ha hb
-  | 3 => this.2.2.2 hc ha hb
+  match i with | 0 => aesop | 1 => aesop | 2 => aesop | 3 => aesop
 
-lemma eq_xor_of_constraints (a b : Vector BabyBear WORD_BYTE_SIZE) (cols : BitwiseOperation)
-    (i : Fin WORD_BYTE_SIZE) (ha : a[i] < 256) (hb : b[i] < 256) (hc : cols.result[i] < 256)
-    (h : (cols.constraints a b 2 1).allHold) :
+lemma eq_xor_of_constraints (a b : ByteWord BabyBear) (cols : BitwiseOperation)
+    (i : Fin WORD_BYTE_SIZE) (h : (cols.constraints a b 2 1).allHold) :
     cols.result[i] = a[i] ^^^ b[i] := by
   have := constraints_imp_spec a b cols _ _ one_ne_zero h
   simp [spec] at this
-  exact match i with
-  | 0 => this.1 hc ha hb
-  | 1 => this.2.1 hc ha hb
-  | 2 => this.2.2.1 hc ha hb
-  | 3 => this.2.2.2 hc ha hb
+  match i with | 0 => aesop | 1 => aesop | 2 => aesop | 3 => aesop
 
 /-- Constraints on `BitwiseOperation` imply that the result is `op.toBitwise` applied to the inputs. -/
-lemma eq_toBitwise_of_constraints (a b : Vector BabyBear WORD_BYTE_SIZE) (cols : BitwiseOperation)
-    (i : Fin WORD_BYTE_SIZE) (ha : a[i] < 256) (hb : b[i] < 256) (hc : cols.result[i] < 256)
-    (op : ByteOpcode) (hop : op = AND ∨ op = OR ∨ op = XOR)
+lemma eq_toBitwise_of_constraints (a b : ByteWord BabyBear) (cols : BitwiseOperation)
+    (i : Fin WORD_BYTE_SIZE) (op : ByteOpcode) (hop : op = AND ∨ op = OR ∨ op = XOR)
     (h : (cols.constraints a b op.toBB 1).allHold) :
     cols.result[i] = op.toBitwise a[i] b[i] := by
   induction op using ByteOpcode.bitwise_induction with
-  | and => exact eq_and_of_constraints _ _ _ _ ha hb hc h
-  | or => exact eq_or_of_constraints _ _ _ _ ha hb hc h
-  | xor => exact eq_xor_of_constraints _ _ _ _ ha hb hc h
+  | and => exact eq_and_of_constraints _ _ _ _ h
+  | or => exact eq_or_of_constraints _ _ _ _ h
+  | xor => exact eq_xor_of_constraints _ _ _ _ h
   | other h h' => aesop
+
+-- lemma lt_of_constraints (a b : ByteWord BabyBear) (cols : BitwiseOperation)
 
 end BitwiseOperation
